---
title: "Template"
pagetitle: "Template"
subtitle: "A template for slides"
author: "Karthik Thiagarajan"
institute: "IIT Madras"
format: revealjs
navigation-mode: vertical
history: false
slide-number: true
show-slide-number: all
incremental: true
fontsize: 30px
margin: 0.1
width: 1600
height: 800
revealjs-plugins:
  - pointer
---

# Measurements

## 

::: {.fragment fragment-index=1 .absolute top=0 left=0}

$\text{top} = 0\\ \text{left} = 0$

:::

::: {.fragment fragment-index=1 .absolute top=0 left=1400}

$\text{top} = 0\\ \text{left} = 1400$

:::

::: {.fragment fragment-index=1 .absolute top=700 left=0}

$\text{top} = 700\\ \text{left} = 0$

:::

::: {.fragment fragment-index=1 .absolute top=700 left=1400}

$\text{top} = 700\\ \text{left} = 1400$

:::

::: {.fragment fragment-index=1 .absolute top=350 left=700}

$\text{top} = 350\\ \text{left} = 700$

:::



## 

::: {.fragment fragment-index=1 .absolute top=0 left=0}

$(0, 0)$

:::

::: {.fragment fragment-index=1 .absolute top=100 left=200}

$(100, 200)$

:::

::: {.fragment fragment-index=1 .absolute top=200 left=400}

$(200, 400)$

:::

::: {.fragment fragment-index=1 .absolute top=300 left=600}

$(300, 600)$

:::

::: {.fragment fragment-index=1 .absolute top=400 left=800}

$(400, 800)$

:::

::: {.fragment fragment-index=1 .absolute top=500 left=1000}

$(500, 1000)$

:::

::: {.fragment fragment-index=1 .absolute top=600 left=1200}

$(600, 1200)$

:::

::: {.fragment fragment-index=1 .absolute top=700 left=1400}

$(700, 1400)$

:::



# Sample Problem

::: {.fragment fragment-index=1 .absolute top=0 left=400}

What is the product of the non-zero eigenvalues of the following matrix:
$$
\begin{bmatrix}
1 & 0 & 0 & 0 & 1\\
0 & 1 & 1 & 1 & 0\\
0 & 1 & 1 & 1 & 0\\
0 & 1 & 1 & 1 & 0\\
1 & 0 & 0 & 0 & 1
\end{bmatrix}
$$

:::



## Solution

::: {.fragment fragment-index=1 .absolute top=200 left=0}

$$
\begin{bmatrix}
1 & 0 & 0 & 0 & 1\\
0 & 1 & 1 & 1 & 0\\
0 & 1 & 1 & 1 & 0\\
0 & 1 & 1 & 1 & 0\\
1 & 0 & 0 & 0 & 1
\end{bmatrix}
$$

:::

::: {.fragment fragment-index=1 .absolute top=-50 left=600}
$$
D = \begin{vmatrix}
1 - \lambda & 0 & 0 & 0 & 1\\
0 & 1 - \lambda & 1 & 1 & 0\\
0 & 1 & 1 - \lambda & 1 & 0\\
0 & 1 & 1 & 1 - \lambda & 0\\
1 & 0 & 0 & 0 & 1 - \lambda
\end{vmatrix}
$$
:::

::: {.fragment fragment-index=1 .absolute top=300 left=400}
$$
D = (1 - \lambda) \begin{vmatrix}
1 - \lambda & 1 & 1 & 0\\
1 & 1 - \lambda & 1 & 0\\
1 & 1 & 1 - \lambda & 0\\
0 & 0 & 0 & 1 - \lambda
\end{vmatrix} + \begin{vmatrix}
0 & 1 - \lambda & 1 & 1\\
0 & 1 & 1 - \lambda & 1\\
0 & 1 & 1 & 1 - \lambda\\
1 & 0 & 0 & 0
\end{vmatrix}
$$
:::

::: {.fragment fragment-index=1 .absolute top=600 left=600}
$$
D = \left[(1 - \lambda)^2 - 1 \right] \begin{vmatrix}
1 - \lambda & 1 & 1\\
1 & 1 - \lambda & 1\\
1 & 1 & 1 - \lambda\\
\end{vmatrix}
$$
:::

::: {.fragment fragment-index=1 .absolute top=600 left=0}
$$
\small
\begin{vmatrix}
1 - \lambda & 1 & 1\\
1 & 1 - \lambda & 1\\
1 & 1 & 1 - \lambda\\
\end{vmatrix} = - \lambda^2 (\lambda - 3)
$$
:::